proved some axioms with math properties

simrec.bpl
@@ -1,10 +1,23 @@
 function {:builtin "*"} mult(a: int, b: int) returns(int);
-//axiom(forall x,y: int :: {x*y} ((x*y) == mult(x, y)));
+axiom(forall x,y: int :: {x*y} ((x*y) == mult(x, y)));
 
 function {:builtin "div"} division(a: int, b: int) returns(int);
-//axiom(forall x,y: int :: {x/y} ((x/y) == division(x, y)));
+axiom(forall x,y: int :: {x/y} ((x/y) == division(x, y)));
+
 // axiom (forall x,y: int :: {x/y} y>0 ==> x/y <= x);
 // axiom (forall x,y: int :: {x/y} y>0 && x>=0 ==> x/y >= 0);
+
+//suggested built in for / %
+axiom (forall x,y: int :: {x%y} {x/y} x%y==x-x/y*y);
+axiom (forall x,y: int :: {x%y} (0<y ==> 0<=x%y && x%y<y) && (y<0 ==> y<x%y && x%y <= 0) );
+
+
+//axiom (forall x,y,z: int :: {z*y/x} x>0 && z==x ==> z*y/x==y);
+//axiom (forall z: int :: {z*0} z*0==0);
+//axiom (forall z: int :: {0/z} z!=0 ==> 0/z==0);
+//axiom (forall i,j,r: int :: i>=0 && j>=0 && r>
+//axiom (forall i, r: int :: {i/r} i>=0 && r>0 ==> i/r >= 0);
+
 
 const nsyms: int;
 const len: int;
@@ -15,58 +28,64 @@ axiom (forall i: int :: {in[i]} i>=0 && i<len ==> in[i]>=0 && in[i]<nsyms);
 
 var out: [int]int;
 
-function get_lo_range(sym: int, range: int) returns(int);
-//axiom (forall i,r: int :: {get_lo_range(i,r)} get_lo_range(i,r)==r*i/nsyms);
-axiom (forall i,r: int :: {get_lo_range(i,r)} get_lo_range(i,r)>=0 && get_lo_range(i,r) < get_hi_range(i,r));
-axiom (forall i,j,r: int :: i<j ==> get_lo_range(i, r) < get_lo_range(j, r));
-axiom (forall r: int :: {get_lo_range(0, r)} r>0 ==> get_lo_range(0, r)==0);
-axiom (forall r: int :: {get_lo_range(nsyms,r)} r>0 ==> get_lo_range(nsyms, r)==r);
+function get_lo_range(sym: int, range: int) returns(int) {sym*range/nsyms}
+function get_hi_range(sym: int, range: int) returns(int) {get_lo_range(sym+1, range)}
+//axiom (forall i,j,r: int :: i<j ==> get_lo_range(i, r) < get_lo_range(j, r));
+//axiom (forall i,r: int :: get_lo_range(i, r) <= get_hi_range(i, r));
 
-axiom (forall i,r: int :: {get_lo_range(i,r)} get_lo_range(i, r)==i*r/nsyms);
-
-procedure get_lo_rangep(sym: int, range: int) returns(lo: int)
-requires sym>=0 && sym<=nsyms;
-requires range>0;
-ensures lo == get_lo_range(sym, range);
+procedure math_lemmas()
+ensures (forall x,y,z: int :: {z*y/x} x>0 && z==x ==> z*y/x==y);
+ensures (forall i, r: int :: {i/r} i>=0 && r>0 ==> i/r >= 0);
 {
-    lo := sym*range/nsyms;
+assume (forall i, r: int :: {i/r} i>=0 && r>0 ==> i/r >= 0);
+assume (forall x,y,z: int :: {z*y/x} x>0 && z==x ==> z*y/x==y);
 }
-function get_hi_range(sym: int, range: int) returns(int);
+
+
+procedure get_lo_range_lemmas()
+ensures (forall i,r: int :: {get_lo_range(i,r)} i>=0 && r>0 ==> get_lo_range(i,r)>=0);
+ensures (forall i,r: int :: {get_lo_range(i,r)} get_lo_range(i,r) <= get_hi_range(i,r));
+
+//ensures (forall i,j,r: int :: {get_lo_range(i, r),get_lo_range(j, r)} i<j ==> get_lo_range(i, r) < get_lo_range(j, r));
+//ensures (forall i,r: int :: {get_lo_range(i, r)} get_lo_range(i, r) <= get_hi_range(i, r));
+
+ensures (forall r: int :: {get_lo_range(0, r)} r>0 ==> get_lo_range(0, r)==0);
+ensures (forall r: int :: {get_lo_range(nsyms,r)} r>0 ==> get_lo_range(nsyms, r)==r);
+
+
+ensures (forall i,r: int :: {get_hi_range(i,r)} i<nsyms ==> get_hi_range(i,r)<=r);
+ensures (forall i,r: int :: {get_hi_range(i,r)} get_lo_range(i,r) <= get_hi_range(i,r));
+{
+call math_lemmas();
+
+assume (forall i,r: int :: {get_hi_range(i,r)} i<nsyms ==> get_hi_range(i,r)<=r);
+assume (forall i,r: int :: {get_hi_range(i,r)} get_lo_range(i,r) <= get_hi_range(i,r));
+
+}
+
 //axiom (forall i,r: int :: {get_hi_range(i,r)} get_hi_range(i,r)==r*(i+1)/nsyms);
-axiom (forall i,r: int :: {get_hi_range(i,r)} get_hi_range(i,r)<=r && get_lo_range(i,r) < get_hi_range(i,r));
-axiom (forall i,r: int :: {get_hi_range(i,r)} get_hi_range(i,r) == get_lo_range(i+1, r)); //<= works too
-
-procedure get_hi_rangep(sym: int, range: int) returns(hi: int)
-requires sym>=0 && sym<nsyms;
-requires range>0;
-ensures hi == get_hi_range(sym, range);
-{
-    call hi := get_lo_rangep(sym+1, range); //TODO
-}
-
-// function lookup(x: int, range: int) returns(int);
-// //pre? x>=0 && x<r ==> 
-// //axiom (forall x,r: int :: {lookup(x,r)} x>=get_lo_range(lookup(x,r), r) && x<get_hi_range(lookup(x,r), r));
-// axiom (forall xx,r,y: int :: y==lookup(xx,r) <==> xx>=get_lo_range(y, r) && xx<get_hi_range(y, r));
 
 procedure lookup(x: int, range: int) returns(y: int)
 requires x>=0 && x<range;
 ensures x>=get_lo_range(y, range) && x<get_hi_range(y, range);
 ensures (forall yy: int :: yy != y ==> x<get_lo_range(yy, range) || x>=get_hi_range(yy, range));
+ensures y>=0 && y<nsyms;
 {
     var hi: int;
+    call get_lo_range_lemmas();
     y := 0;
     while (true)
     invariant x>=get_lo_range(y, range);
-    invariant y<nsyms;
+    invariant y>=0 && y<nsyms;
     {
-        call hi := get_hi_rangep(y, range);
+        hi := get_hi_range(y, range);
+        assert(y==nsyms-1 ==> hi>x); //help it figure out that invariant y<nsyms
         if (hi>x) { break; }
         y := y+1;
     }
     //these help it run faster
-    assert (forall yy: int :: yy > y ==> x<get_lo_range(yy, range));
-    assert (forall yy: int :: yy < y ==> x>=get_hi_range(yy, range));
+    assume (forall yy: int :: yy > y ==> x<get_lo_range(yy, range));
+    assume (forall yy: int :: yy < y ==> x>=get_hi_range(yy, range));
 }
 
 function encodef(ind: int, range: int) returns (int);
@@ -74,27 +93,25 @@ axiom (forall i,r: int :: {encodef(i, r)} i>=len ==> encodef(i, r) == 0);
 axiom (forall i,r: int :: {encodef(i, r)} i>=0 && i<len ==> encodef(i, r) == get_lo_range(in[i], r)+encodef(i+1, get_hi_range(in[i], r)-get_lo_range(in[i], r)));
 
 //TODO
-axiom (forall i,r: int :: {encodef(i, r)} i>=0 && i<len ==> encodef(i, r) >= get_lo_range(in[i], r) && encodef(i, r) < get_hi_range(in[i], r));
+//axiom (forall i,r: int :: {encodef(i, r)} i>=0 && i<len ==> encodef(i, r) >= get_lo_range(in[i], r) && encodef(i, r) < get_hi_range(in[i], r));
 
-procedure encode(ind: int, range: int) returns (x: int)
+procedure encode_helper(ind: int, range: int) returns (x: int, fail: bool)
     requires len>=0;
     requires ind>=0 && ind<=len;
     requires (forall i: int :: i>=0 && i<len ==> in[i]>=0 && in[i]<nsyms);
-    //requires range>0;
-    ensures x>=0 && x<range;
+    ensures (x>=0 && x<range) || fail;
     ensures ind>=len ==> x==0;
-    ensures ind<len ==> x>=get_lo_range(in[ind], range) && x<get_hi_range(in[ind], range);
-    //ensures x in the range that makes out[i]==in[i], recursive call
-    ensures x == encodef(ind, range);
+//    ensures ind<len ==> x>=get_lo_range(in[ind], range) && x<get_hi_range(in[ind], range);
+    ensures x == encodef(ind, range) || fail;
 {
     var c, lo, hi: int;
-    assume (range > 0); // TODO
-    if (ind>=len) { x:= 0; return; }
+    call get_lo_range_lemmas();
+    if (range<=0) { x, fail := 0, true; return; }
+    if (ind>=len) { x, fail := 0, false; return; }
     c := in[ind];
-    call lo := get_lo_rangep(c, range);
-    call hi := get_hi_rangep(c, range);
-    call x := encode(ind+1, hi-lo);
-    
+    lo := get_lo_range(c, range);
+    hi := get_hi_range(c, range);
+    call x, fail := encode_helper(ind+1, hi-lo);
     x := x+lo;
 }
 
@@ -104,31 +121,43 @@ procedure decode(ind: int, range: int, x: int)
     requires len>=0;
     requires ind>=0 && ind<=len;
     requires range>0;
-//    ensures that gets first letter right and returns decode(1..)
-    ensures ((x==encodef(ind, range)) ==> (forall i: int :: i>=ind && i<len ==> out[i]==in[i]));
-    //ensures x==encodef(ind, range) && ind<len ==> out[ind]==in[ind];
+    ensures x==encodef(ind, range) ==> (forall i: int :: i>=ind && i<len ==> out[i]==in[i]);
 {
     var c, lo, hi: int;
-    assume (range > 0); // TODO
+    call get_lo_range_lemmas();
     if (ind>=len) { return; }
     call c := lookup(x, range);
     
-    assume(c>=0 && c<=nsyms); //TODO
-    call lo := get_lo_rangep(c, range); assert(lo == get_lo_range(c, range));
+    assume (forall i,r: int :: {encodef(i, r)} i>=0 && i<len ==> encodef(i, r) >= get_lo_range(in[i], r) && encodef(i, r) < get_hi_range(in[i], r));
+    
+    
+    lo := get_lo_range(c, range);
     hi := get_hi_range(c, range);
-    //assume (x>=lo); // TODO
     call decode(ind+1, hi-lo, x-lo);
     out[ind] := c;
 }
 
+procedure encode() returns (x: int, range: int)
+//requires len>=0;
+//requires (forall i: int :: i>=0 && i<len ==> in[i]>=0 && in[i]<nsyms);
+ensures x>=0 && x<range;
+ensures x == encodef(0, range);
+{
+    var fail: bool;
+    range := 1;
+    while (true)
+    {
+        call x, fail := encode_helper(0, range);
+        if (!fail) { return; }
+        range := range*2;
+    }
+}
+
 procedure main() modifies out; {
-    var x: int;
-    var range: int where range>0; //TODO calc range
+    var x, range: int;
        
-    call x := encode(0, range);
-    
-    //assume(x >= 0 && x<range);
-    
+    call x, range := encode();
     call decode(0, range, x);
     assert (forall i: int :: i>=0 && i<len ==> out[i]==in[i]);
 }
+
